Add back index to sdcs.
sdcs_cofinite_switch describe the issue with cofinite quantification and
existential index, but moving on.

cc @TiarkRompf

cln/MuDotX.v
@@ -425,7 +425,7 @@ Inductive stp: nat -> bool -> ctx -> typ -> typ -> ctx -> Prop :=
   G2 = G2A & G2B & G2C ->
   G2X = G2A & G2C ->
   (forall x, x \notin L ->
-   sdcs
+   sdcs n1
         (G1X & (x ~ typ_clo G1X (typ_bind Ds1)))
         (open_decs x Ds1)
         (open_decs x Ds2)
@@ -459,16 +459,16 @@ with sdc: nat -> ctx -> dec -> dec -> ctx -> Prop :=
   stp n2 true G1 TU1 TU2 G2 ->
   sdc (S (n1+n2)) G1 (dec_mtd m TL1 TU1) (dec_mtd m TL2 TU2) G2
 
-with sdcs: ctx -> decs -> decs -> ctx -> Prop :=
-| sdcs_nil: forall G1 Ds1 G2,
+with sdcs: nat -> ctx -> decs -> decs -> ctx -> Prop :=
+| sdcs_nil: forall n1 G1 Ds1 G2,
   wf_decs G1 Ds1 ->
-  sdcs G1 Ds1 decs_nil G2
-| sdcs_cons: forall n1 G1 Ds1 G2 Ds2 D1 D2,
+  sdcs (S n1) G1 Ds1 decs_nil G2
+| sdcs_cons: forall n1 n2 G1 Ds1 G2 Ds2 D1 D2,
   decs_has Ds1 D1 ->
   sdc n1 G1 D1 D2 G2 ->
-  sdcs G1 Ds1 Ds2 G2 ->
+  sdcs n2 G1 Ds1 Ds2 G2 ->
   decs_hasnt Ds2 (label_of_dec D2) ->
-  sdcs G1 Ds1 (decs_cons D2 Ds2) G2
+  sdcs (S (n1+n2)) G1 Ds1 (decs_cons D2 Ds2) G2
 
 with wf_typ: ctx -> typ -> Prop :=
 | wf_sel: forall n1 G p M TL TU Gp,
@@ -512,6 +512,7 @@ with wf_decs: ctx -> decs -> Prop :=
 
 Definition stpn b G1 T1 T2 G2 := exists n, stp n b G1 T1 T2 G2.
 Definition sdcn G1 D1 D2 G2 := exists n, sdc n G1 D1 D2 G2.
+Definition sdcsn G1 Ds1 Ds2 G2 := exists n, sdcs n G1 Ds1 Ds2 G2.
 
 Inductive tc_trm: ctx -> trm -> typ -> Prop :=
 | tc_var: forall G T x Gx Tx,
@@ -626,7 +627,7 @@ Combined Scheme ep_mutind from exp_mut_ep, pth_has_mut_ep.
 Theorem sub_reg:
   (forall n b G1 T1 T2 G2, stp n b G1 T1 T2 G2 -> wf_typ G1 T1 /\ wf_typ G2 T2) /\
   (forall n G1 D1 D2 G2, sdc n G1 D1 D2 G2 -> wf_dec G1 D1 /\ wf_dec G2 D2) /\
-  (forall G1 Ds1 Ds2 G2, sdcs G1 Ds1 Ds2 G2 -> wf_decs G1 Ds1 /\ wf_decs G2 Ds2).
+  (forall n G1 Ds1 Ds2 G2, sdcs n G1 Ds1 Ds2 G2 -> wf_decs G1 Ds1 /\ wf_decs G2 Ds2).
 Proof.
   apply sub_mutind; intros.
   - (* T1 <: p.M -- sel2 *)
@@ -710,11 +711,11 @@ Proof.
   apply (proj2 (sdc_reg H)).
 Qed.
 
-Lemma sdcs_reg1: forall G1 Ds1 Ds2 G2,
-  sdcs G1 Ds1 Ds2 G2 ->
+Lemma sdcs_reg1: forall n G1 Ds1 Ds2 G2,
+  sdcs n G1 Ds1 Ds2 G2 ->
   wf_decs G1 Ds1.
 Proof.
-  intros G1 Ds1 Ds2 G2 H.
+  intros n G1 Ds1 Ds2 G2 H.
   apply (proj1 (sdcs_reg H)).
 Qed.
 
@@ -731,11 +732,11 @@ Proof.
     - apply IHdecs_hasnt. assumption.
 Qed.
 
-Lemma sdcs_cons1: forall G1 Ds1 Ds2 G2 D1,
-  sdcs G1 Ds1 Ds2 G2 ->
+Lemma sdcs_cons1: forall n G1 Ds1 Ds2 G2 D1,
+  sdcs n G1 Ds1 Ds2 G2 ->
   wf_dec G1 D1 ->
   decs_hasnt Ds1 (label_of_dec D1) ->
-  sdcs G1 (decs_cons D1 Ds1) Ds2 G2.
+  sdcs n G1 (decs_cons D1 Ds1) Ds2 G2.
 Proof.
   intros.
   induction H.
@@ -748,13 +749,29 @@ Proof.
     - assumption.
 Qed.
 
+(* Problem with cofinite quantification and index-based induction scheme. *)
+Axiom sdcs_cofinite_switch: forall L Ds1 Ds2 G1X G2X,
+  (forall x, x \notin L ->
+   sdcsn
+        (G1X & (x ~ typ_clo G1X (typ_bind Ds1)))
+        (open_decs x Ds1)
+        (open_decs x Ds2)
+        (G2X & (x ~ typ_clo G1X (typ_bind Ds1)))) ->
+  exists n,
+  (forall x, x \notin L ->
+   sdcs n
+        (G1X & (x ~ typ_clo G1X (typ_bind Ds1)))
+        (open_decs x Ds1)
+        (open_decs x Ds2)
+        (G2X & (x ~ typ_clo G1X (typ_bind Ds1)))).
+
 Theorem sub_refl:
   (forall n b G1 T1 T2 G2, stp n b G1 T1 T2 G2 -> stpn b G1 T1 T1 G1 /\ stpn b G2 T2 T2 G2) /\
   (forall n G1 D1 D2 G2, sdc n G1 D1 D2 G2 -> sdcn G1 D1 D1 G1 /\ sdcn G2 D2 D2 G2) /\
-  (forall G1 Ds1 Ds2 G2, sdcs G1 Ds1 Ds2 G2 -> sdcs G1 Ds1 Ds1 G1 /\ sdcs G2 Ds2 Ds2 G2) /\
+  (forall n G1 Ds1 Ds2 G2, sdcs n G1 Ds1 Ds2 G2 -> sdcsn G1 Ds1 Ds1 G1 /\ sdcsn G2 Ds2 Ds2 G2) /\
   (forall G T, wf_typ G T -> stpn true G T T G) /\
   (forall G D, wf_dec G D -> sdcn G D D G) /\
-  (forall G Ds, wf_decs G Ds -> sdcs G Ds Ds G).
+  (forall G Ds, wf_decs G Ds -> sdcsn G Ds Ds G).
 Proof.
   apply sw_mutind; intros.
   - (* T1 <: p.M -- sel2 *)
@@ -807,16 +824,21 @@ Proof.
       apply same_rfl.
   - (* bind *)
     split.
-    + exists (S 0).
+    + assert (forall x, x \notin L ->
+       sdcsn (G1X & x ~ typ_clo G1X (typ_bind Ds1))
+         (open_decs x Ds1) (open_decs x Ds1)
+         (G1X & x ~ typ_clo G1X (typ_bind Ds1))) as A. {
+        intros x Fr. specialize (H0 x Fr). inversion H0.
+        assumption.
+      }
+      apply sdcs_cofinite_switch in A. inversion A as [n' A'].
+      exists (S n').
       apply stp_bind with (L:=L)
         (G1A:=G1A) (G1B:=G1B) (G1C:=G1C) (G1X:=G1X)
-        (G2A:=G1A) (G2B:=G1B) (G2C:=G1C) (G2X:=G1X).
+        (G2A:=G1A) (G2B:=G1B) (G2C:=G1C) (G2X:=G1X); auto.
       apply wf_bind with (L:=L)
-        (GA:=G1A) (GB:=G1B) (GC:=G1C) (GX:=G1X).
-      assumption. assumption.
+        (GA:=G1A) (GB:=G1B) (GC:=G1C) (GX:=G1X); auto.
       intros x Frx. eapply sdcs_reg1. specialize (s x Frx). apply s.
-      assumption. assumption. assumption. assumption.
-      intros x Frx. specialize (H0 x Frx). inversion H0. assumption.
     + assumption.
   - (* transf *)
     split.
@@ -860,12 +882,13 @@ Proof.
   - (* Ds1 <: {} -- nil *)
     split.
     + assumption.
-    + apply sdcs_nil. apply wf_decs_nil.
+    + exists (S 0). apply sdcs_nil. apply wf_decs_nil.
   - (* Ds1 <: D2::Ds2 -- cons *)
     split.
     + inversion H0. assumption.
-    + inversion H0 as [_ HDs2].
+    + inversion H0 as [_ HDs2]. inversion HDs2 as [n2' HDs2'].
       inversion H as [_ HD2]. inversion HD2 as [n1' HD2'].
+      exists (S (n1'+n2')).
       apply sdcs_cons with (D1:=D2) (n1:=n1').
         apply decs_has_hit; assumption.
         assumption.
@@ -883,7 +906,8 @@ Proof.
     apply stp_selxu with (TU1:=TU) (TU2:=TU) (Gp1:=Gp) (Gp2:=Gp);
     try assumption; try solve [apply same_rfl].
   - (* wf_bind *)
-    exists (S 0).
+    apply sdcs_cofinite_switch in H. inversion H as [n' H'].
+    exists (S n').
     apply stp_bind with (L:=L)
       (G1A:=GA) (G1B:=GB) (G1C:=GC) (G1X:=GX)
       (G2A:=GA) (G2B:=GB) (G2C:=GC) (G2X:=GX);
@@ -907,9 +931,11 @@ Proof.
     apply sdc_mtd; try assumption.
     apply stp_wrapf. assumption.
   - (* wf_decs_nil *)
-    apply sdcs_nil. apply wf_decs_nil.
+    exists (S 0). apply sdcs_nil. apply wf_decs_nil.
   - (* wf_decs_cons *)
+    inversion H0 as [n2 HDs'].
     inversion H as [n1 HD'].
+    exists (S (n1+n2)).
     apply sdcs_cons with (D1:=D) (n1:=n1); try assumption.
     + apply decs_has_hit. assumption.
     + apply sdcs_cons1; try assumption.
@@ -942,11 +968,11 @@ Theorem sub_extending:
      G2 = G2A & G2C ->
      sdc n (G1A & G1B & G1C) D1 D2 (G2A & G2B & G2C)
   ) /\
-  (forall G1 Ds1 Ds2 G2, sdcs G1 Ds1 Ds2 G2 ->
+  (forall n G1 Ds1 Ds2 G2, sdcs n G1 Ds1 Ds2 G2 ->
    forall G1A G1B G1C G2A G2B G2C,
      G1 = G1A & G1C ->
      G2 = G2A & G2C ->
-     sdcs (G1A & G1B & G1C) Ds1 Ds2 (G2A & G2B & G2C)
+     sdcs n (G1A & G1B & G1C) Ds1 Ds2 (G2A & G2B & G2C)
   ) /\
   (forall G T, wf_typ G T ->
    forall GA GB GC,
@@ -1233,24 +1259,6 @@ Proof.
   eapply stp_sel1u; try eassumption.
 Qed.
 
-Lemma sdcs_trans: forall x Ds1 Ds2 Ds3 G1A G2B G1C G2A G2C G1A0 G1B0 G1C0 G2A0 G2C0,
-   G2A & G2B & G2C = G1A0 & G1B0 & G1C0 ->
-   sdcs (G1A & G1C & x ~ typ_clo (G1A & G1C) (typ_bind Ds1))
-        (open_decs x Ds1) (open_decs x Ds2)
-        (G2A & G2C & x ~ typ_clo (G1A & G1C) (typ_bind Ds1))
-   ->
-   sdcs (G1A0 & G1C0 & x ~ typ_clo (G1A0 & G1C0) (typ_bind Ds2))
-        (open_decs x Ds2) (open_decs x Ds3)
-        (G2A0 & G2C0 & x ~ typ_clo (G1A0 & G1C0) (typ_bind Ds2))
-   ->
-   sdcs (G1A & G1C & x ~ typ_clo (G1A & G1C) (typ_bind Ds1))
-     (open_decs x Ds1) (open_decs x Ds3)
-     (G2A0 & G2C0 & x ~ typ_clo (G1A & G1C) (typ_bind Ds1))
-   .
-Proof.
-  admit.
-Qed.
-
 Lemma stp_trans: forall n, trans_up n.
 Proof.
   intros n. induction n.
@@ -1430,13 +1438,13 @@ Proof.
 
   + (* bind - bind *)
     inversions H19.
-    exists (S 0).
+    exists (S n).
     apply stp_bind with (L:=L \u L0) (G1A:=G1A) (G1B:=G1B) (G1C:=G1C) (G1X:=G1A & G1C) (G2A:=G2A0) (G2B:=G2B0) (G2C:=G2C0) (G2X:=G2A0 & G2C0); try assumption; try reflexivity.
     intros x Frx.
     assert (x \notin L) as FrL by auto.
     assert (x \notin L0) as FrL0 by auto.
     specialize (H4 x FrL). specialize (H15 x FrL0).
-    eapply sdcs_trans; eassumption.
+    admit.
 Qed.
 
 Theorem trans: forall G1 T1 G2 T2 G3 T3,
